\documentclass{article}
\usepackage[margin=1.0in]{geometry}
\usepackage{amssymb,amsmath,amsthm,amsfonts}
\usepackage{enumitem}
\usepackage{xcolor}
\usepackage{mathtools}
\usepackage{booktabs,float}

% My boxes
\usepackage[breakable]{tcolorbox}

% \RequirePackage{background}
% \backgroundsetup{
%     scale=1,
%     color=black,
%     opacity=1,
%     angle=0,
%     contents={
%         \includegraphics[width=\paperwidth,height=\paperheight]{\nightmodebackground}
%     }
% }

\definecolor{pastelblue}{RGB}{96, 145, 245}
\definecolor{pastelgreen}{RGB}{106, 235, 135}
\definecolor{darkgray}{RGB}{60, 60, 60}
\definecolor{lightgray}{RGB}{180, 180, 180}
\definecolor{offwhite}{RGB}{225, 225, 245}


\pagecolor{darkgray}
\color{offwhite}

\newcommand{\Z}{\mathbf{Z}}
\newcommand{\N}{\mathbf{N}}
\newcommand{\R}{\mathbf{R}}
\newcommand{\Q}{\mathbf{Q}}
\newcommand{\C}{\mathbf{C}}

\newcommand{\id}{\mathrm{id}}
\newcommand{\op}{\mathrm{op}}
\newcommand{\diam}{\mathrm{diam}}
\newcommand{\GL}{\mathrm{GL}}
\newcommand{\Tr}{\mathrm{Tr}}
\newcommand{\im}{\mathrm{im}}
\newcommand{\rank}{\mathrm{rank}}

\newcommand{\cl}[1]{\overline{#1}}

\swapnumbers % places numbers before thm names

\theoremstyle{plain} % The "plain" style italicizes all body text.
	\newtheorem{thm}{Theorem}
		\numberwithin{thm}{section} % Theorem numbers are determined by section.
	\newtheorem{lemma}[thm]{Lemma}
	\newtheorem{prop}[thm]{Proposition}
	\newtheorem{cor}[thm]{Corollary}

\theoremstyle{definition}
    \newtheorem{defn}[thm]{Definition}
	\newtheorem{example}[thm]{Example}
	\newtheorem{exercise}[thm]{Exercise} %Exercise

\begin{document}
    \newtcolorbox{question}[2][]{fonttitle=\large, fontupper=\large, fontlower=\large, title=Question {#2}., oversize, arc=3mm, outer arc=2mm, opacityback=0.9, coltitle=offwhite, colframe=pastelblue, colback=darkgray, colupper=lightgray, collower=lightgray, leftrule=1mm, rightrule=1mm, toprule=1.5mm, titlerule=1mm, bottomrule=1mm, valign=center, add to natural height=5mm, lower separated=false, before lower=\begin{proof}, after lower= \smallbreak \end{proof}, #1, breakable=true}

    \begin{question}{1}
        Find all solutions to the following complex equations.
        \begin{enumerate}
            \item \((1 + i)\cl{z} = i(2 + 8i)\)
            \item \(z^3 = -8i\)
            \item \(e^{\cl{z}} = -2 + 2i\)
        \end{enumerate}
        \tcblower
        \ 
        \begin{enumerate}
            \item \((1+i)\cl{z} = i(2 + 8i)\).
            
            Suppose that \(z\) is of the form \(z = a + bi\), for \(a,b \in \mathbb{R}\). Then the equation becomes
            \[
                (1+i)(a - bi) = i(2 + 8i) \implies a + b + (a - b)i = -8 + 2i.
            \]
            Equating coefficients, we get
            \[
                a + b = -8 \text{ and } a - b = 2.
            \]
            Solving the system of equations gives us \(a = -3\) and \(b = -5\), so \(z = -3 - 5i\).

            \item \(z^3 = -8i\).
            
            Suppose that \(z\) is of the form \(z = re^{i \theta}\), for \(r, \theta \in \mathbb{R}\). Then the equation becomes
            \[
                r^3 e^{3i \theta} = -8i \implies r^3 e^{3i \theta} = 8e^{-i \left( \frac{\pi}{2} + 2n\pi  \right)} \text{, for } n \in \mathbb{Z}
            \]
            Equating the coefficient and exponent gives us
            \[
                r^3 = 8 \text{ and } 3\theta = \frac{\pi}{2} + 2n \pi \implies r = 2,\ \theta = \frac{\pi}{6} + \frac{2n \pi}{3}.
            \]
            Therefore
            \[
                z = 2e^{i\left( \frac{\pi}{6} + \frac{2n \pi}{3}\right)} = 2\cos \left( \frac{\pi}{6} + \frac{2n \pi}{3} \right) + 2i\sin \left( \frac{\pi}{6} + \frac{2n \pi}{3} \right).
            \]
            We can convert this into the standard form by considering cases when \(n = 0,1,2\), as any other value will give us a value of \(z\) that is already accounted for. Therefore
            \[
                z = \sqrt{3} + i, -\sqrt{3} + i, -2i
            \]



            \item \(e^{\cl{z}} = -2 + 2i\).
            
            Let \(z = a + bi\), for \(a,b \in \mathbb{R}\). Converting the right hand side of the equation into polar form, we get
            \[
                e^a e^{bi} = 2\sqrt{2} e^{i \left(\frac{3\pi} {4} + 2n \pi \right)}, \text{ where } n \in \mathbb{Z}.
            \]
            We can equate real and complex parts to get that
            \[
                e^a = 2\sqrt{2} \text{ and } b = \frac{3\pi}{4} + 2n \pi
            \]
            so
            \[
                z = \frac{3}{2}\ln (2) + i\left( \frac{3\pi}{2} + 2n \pi\right).
            \]
        \end{enumerate}
    \end{question}
    \newpage
    \begin{question}{2}
        Find all solutions to the following equations in \( \mathbb{Z}_9 \), or show that they have no solution.

        \begin{enumerate}
            \item[(a)] \([4]x + [3] = [1]\)
            \item[(b)] \([6]x + [3] = [5]\)
            \item[(c)] \(x^2 = [0]\).
        \end{enumerate}
        \tcblower
        \begin{enumerate}
            \item[(a)] \([4]x + [3] = [1]\)
            
            Adding \([6]\) to both sides of the equation yields
            \[
                [4]x = [7].
            \]
            Multiplying both sides by \([7]\), we get
            \[
                [28]x = [49]
            \]
            \[
                \implies x = [4].
            \]
            
            \item[(b)] \([6]x + [3] = [5]\)
            
            This equation has no solution. To show this, we first simplify the equation to \([6]x = [2]\) by adding \([6]\) to both sides. We can substitute \(x = [0], ..., [8]\) into the left hand side and see that it does not equal the right hand side:
            \[
                [6][1] = [6],\ [6][2] = [3],\ [6][3] = [0],\ [6][4] = [6],\ [6][5] = [3],\ [6][6] = [0],\ 
            \]
            \[
                [6][7] = [6],\ [6][8] = [3],\ 
            \]
            As shown, the left hand side can never equal \([5]\), so the equation has no solution.

            \item[(c)] \(x^2 = [0]\)
            
            We can solve this by substituting every element in \(\mathbb{Z}_9\) into the left hand side. We see that
            \[
                [0]^2 = [0],\ [1]^2 = [1],\ [2]^2 = [4],\ [3]^2 = [0],\ [4]^2 = [7],\ 
            \]
            \[
                [5]^2 = [7],\ [6]^2 = [0],\ [7]^2 = [4],\ [8]^2 = [1].
            \]
            Thus the solutions to this equation are \(x = [0], [3], [6]\).
        \end{enumerate}
    \end{question}
    \newpage
    \begin{question}{3}
        Let \( \mathbb{Z}_3[i] = \{ a + bi \mid a, b \in \mathbb{Z}_3 \} \), where we define operations \( +, \cdot \) by:

        \[
        (a + bi) + (c + di) = (a + c) + (b + d)i
        \]

        \[
        (a + bi) \cdot (c + di) = (ac - bd) + (ad + bc)i.
        \]

        Set \( 1 = [1] + [0]i \) and \( 0 = [0] + [0]i \).

        \begin{enumerate}
            \item[(a)] Using only the definition of the operations above, and the fact that \( \mathbb{Z}_3 \) is a field, show that \( \mathbb{Z}_3[i] \) satisfies Axioms 1-4, as well as the existence of additive inverses.
            
            \item[(b)] Compute the multiplication table for \( \mathbb{Z}_3[i] \) to verify that multiplicative inverses exist, and hence conclude that \( \mathbb{Z}_3[i] \) is a field.
            
            \item[(c)] What is the characteristic of \( \mathbb{Z}_3[i] \)? (See question \#6 for the definition of characteristic of a field.)
        \end{enumerate}
        \tcblower
        \ 

        (a):

        Let \(a,b,c,d,p,q \in \mathbb{Z}_3\), so \(z = a + bi\), \(w = c + di\), and \(x = p + qi\) are elements of \(\mathbb{Z}_3[i]\).

        \smallbreak

        To show closure under addition and multiplication, we use the closure of \(\mathbb{Z}_3\) to see that \(a + c \in \mathbb{Z}_3\) and \(b + d \in \mathbb{Z}_3\). It follows that \(z + w = (a + c) + (b + d)i \in \mathbb{Z}_3[i]\).

        As well, we also have that \(ac - bd, ad + bc \in \mathbb{Z}_3\), so \(zw = (ac - bd) + (ad  +bc)i \in \mathbb{Z}_3[i]\).

        \smallbreak

        To show the commutativity of addition and multiplication, we note that \(a + c = c + a\) and \(b + d = d + b\), so
        \[
            z + w = (a + c) + (b + d)i = (c + a) + (d + b)i = w + z
        \]
        Likewise, since \(ac = ca\), \(bd = db\), \(ad = da\), and \(bc = cb\),
        \[
            zw = (ac - bd) + (ad + bc)i = (ca - db) + (da + cb)i = wz
        \]

        \smallbreak

        To show associativity, we again use the field properties of \(\mathbb{Z}_3\) to see that
        \begin{align*}
            (z + w) + x &= ((a + c) + (b + d)i) + p + qi \\
            &= ((a + c) + p) + ((b + d) + q)i \\
            &= (a + (c + p)) + (b + (d + q))i \tag{associativity of \(\mathbb{Z}_3\)} \\
            &= a + bi + (c + p) + (d + q)i \\
            &= z + (w + x)
        \end{align*}

        \smallbreak

        Finally, showing distributivity, we have
        \begin{align*}
            x \cdot (z + w) &= (p + qi) \cdot ((a + c) + (b + d)i) \\
            &= p(a + c) - q(b + d) + (p(b + d) + q(a + c))i \\
            &= pa + pc - qb - qd + (pb + pd + qa + qc)i \tag{distributivity of \(\mathbb{Z}_3\)} \\
            &= (pa - qb) + (pc - qd) + ((pb + qa) + (pd + qc))i \tag{associativity \& commutativity of \(\mathbb{Z}_3\)} \\
            &= (pa - qb) + (pb + qa)i + (pc - qd) + (pd + qc)i \\
            &= (p + qi) \cdot (a + bi) + (p + qi) \cdot (c + di) \\
            &= x \cdot z + x \cdot w
        \end{align*}

        We also see that additive inverses exist, because for \(z = a + bi \in \mathbb{Z} _3[i]\), we know that \(-a\) and \(-b\) exist, so if we let \(-z = (-a) + (-b)i\), we see that
        \begin{align*}
            z + (-z) &= (a + bi) + (-a + (-b)i) \\
            &= (a + (-a)) + (b + (-b))i \\
            &= 0 + 0i \\
            &= 0
        \end{align*}

        \medskip

        (b):

        Below is the multiplication table for \(\mathbb{Z}_3[i]\):
        \begin{table}[H]
            \centering
            \begin{tabular}{c|c|c|c|c|c|c|c|c|c}
                \toprule
                    & \(0 + 0i\) & \(1 + 0i\) & \(2 + 0i\) & \(0 + 1i\) & \(1 + 1i\) & \(2 + 1i\) & \(0 + 2i\) & \(1 + 2i\) & \(2 + 2i\) \\
                \midrule
                    \(0 + 0i\) & 0 & 0 & 0 & 0 & 0 & 0 & 0 & 0 & 0 \\
                    \(1 + 0i\) & 0 & \(1 + 0i\) & \(2 + 0i\) & \(0 + 1i\) & \(1 + 1i\) & \(2 + 1i\) & \(0 + 2i\) & \(1 + 2i\) & \(2 + 2i\) \\
                    \(2 + 0i\) & 0 & \(2 + 0i\) & \(1 + 0i\) & \(0 + 2i\) & \(2 + 2i\) & \(1 + 2i\) & \(0 + 1i\) & \(2 + 1i\) & \(1 + 1i\) \\
                    \(0 + 1i\) & 0 & \(0 + 1i\) & \(0 + 2i\) & \(2 + 0i\) & \(2 + 1i\) & \(2 + 2i\) & \(1 + 0i\) & \(1 + 1i\) & \(1 + 2i\) \\
                    \(1 + 1i\) & 0 & \(1 + 1i\) & \(2 + 2i\) & \(2 + 1i\) & \(0 + 2i\) & \(1 + 0i\) & \(1 + 2i\) & \(2 + 0i\) & \(0 + 1i\) \\
                    \(2 + 1i\) & 0 & \(2 + 1i\) & \(1 + 2i\) & \(2 + 2i\) & \(1 + 0i\) & \(0 + 2i\) & \(1 + 1i\) & \(0 + i\) & \(2 + 0i\) \\
                    \(0 + 2i\) & 0 & \(0 + 2i\) & \(0 + 1i\) & \(1 + 0i\) & \(1 + 2i\) & \(1 + 1i\) & \(2 + 0i\) & \(2 + 2i\) & \(2 + 1i\) \\
                    \(1 + 2i\) & 0 & \(1 + 2i\) & \(2 + 1i\) & \(1 + 1i\) & \(2 + 0i\) & \(0 + i\) & \(2 + 2i\) & \(0 + 2i\) & \(1 + 0i\) \\
                    \(2 + 2i\) & 0 & \(2 + 2i\) & \(1 + 1i\) & \(1 + 2i\) & \(0 + 1i\) & \(2 + 0i\) & \(2 + 1i\) & \(1 + 0i\) & \(0 + 2i\) \\
                \bottomrule
            \end{tabular}
            \caption{Multiplication table}
            \label{tab:e}
        \end{table}

        As seen, every row and column not belonging to \(0\) contains \(1 + 0i\), which implies that for all \(z \in \mathbb{Z}_3[i]\setminus {0}\), there is a multiplicative inverse \(z^{-1}\).

        \medskip

        (c):
        \(\mathrm{char}(\mathbb{Z}_3[i]) = 3\), as
        \begin{align*}
            1 + 1 + 1 &= ([1] + [0]i) + ([1] + [0]i) + ([1] + [0]i) \\
            &= ([1] + [1] + [1]) + ([0] + [0] + [0])i \\
            &= [0] + [0]i \\
            &= 0
        \end{align*}
    \end{question}
    \newpage
    \begin{question}{4}
        We introduce a new definition in this question:

        \textbf{Definition:} Let \( \mathbb{F} \) be a field. We say a subset \( \mathbb{K} \subseteq \mathbb{F} \) is a \textbf{subfield} of \( \mathbb{F} \) if \( \mathbb{K} \) is also a field, using the same operations as \( \mathbb{F} \).

        For example: \( \mathbb{Q} \) is a subfield of \( \mathbb{R} \). \( \mathbb{R} \) is a subfield of \( \mathbb{C} \). \( \mathbb{Z}_3 \) is not a subfield of \( \mathbb{Q} \), since \( \mathbb{Z}_3 \) is not a subset of \( \mathbb{Q} \).

        \begin{enumerate}
            \item[(a)] Let \( \mathbb{K} \subseteq \mathbb{F} \) be a subfield. Let \( 0_{\mathbb{F}}, 1_{\mathbb{F}} \) denote the additive and multiplicative identities in \( \mathbb{F} \). Similarly, we denote by \( 0_{\mathbb{K}}, 1_{\mathbb{K}} \) the identities in \( \mathbb{K} \). Prove that \( 0_{\mathbb{F}} = 0_{\mathbb{K}} \) and \( 1_{\mathbb{F}} = 1_{\mathbb{K}} \). 
            (Hint: Prove that in a field, the only solution to the equation \( x^2 = x \) are \( x = 0, x = 1 \).)
            
            \item[(b)] Let \( \mathbb{K} \subseteq \mathbb{F} \) be a subfield. Prove that for all \( x \in \mathbb{K} \), we have \( -x \in \mathbb{K} \), and that for all \( x \in \mathbb{K} \setminus \{0\} \) we have \( x^{-1} \in \mathbb{K} \). (Here \( -x \) is the additive inverse of \( x \) \textbf{treated as an element of} \( \mathbb{F} \) and \( x^{-1} \) is the multiplicative inverse of \( x \) \textbf{treated as an element of} \( \mathbb{F} \).)
            
            \item[(c)] Prove that a subset \( \mathbb{K} \subseteq \mathbb{F} \) is a subfield if and only if the following conditions are met:
            
            \begin{enumerate}
                \item[(i)] \( 0,1 \in \mathbb{K} \).
                \item[(ii)] For all \( x, y \in \mathbb{K} \), we have \( x + y, x \cdot y \in \mathbb{K} \).
                \item[(iii)] For all \( x \in \mathbb{K} \), we have \( -x \in \mathbb{K} \).
                \item[(iv)] For all \( x \in \mathbb{K} \setminus \{ 0 \} \), we have \( x^{-1} \in \mathbb{K} \).
            \end{enumerate}
            
            (Hints: For the \( \implies \) direction: this is ``part c'' for a reason. For the \( \impliedby \) direction, you only need one or two short sentences to argue why addition and multiplication in \( \mathbb{K} \) satisfy Axioms 1-3. Axioms 4 and 5 should also have fairly short proofs. If you find yourself with a very long argument, you should rethink your argument.)
            
        \end{enumerate}
        \tcblower
        \ 

        (a):

        Fix \(x \in \mathbb{K}\). Then because \(x \in \mathbb{F}\),
        \[
            0_{\mathbb{F}} + x = x = 0_{\mathbb{K}} + x \tag{existence of additive identity in \( \mathbb{F}\) and \(\mathbb{K}\)}
        \]
        \[
            \implies 0_{\mathbb{F}} = 0_{\mathbb{K}} \tag{by cancellation}
        \]

        Similarly for multiplication,
        \[
            1_{\mathbb{F}} \cdot x = x = 1_{\mathbb{K}} \cdot x \implies 1_{\mathbb{F}} = 1_{\mathbb{K}}
        \]

        \medskip

        (b):

        Let \(x \in \mathbb{K}\). Since \(\mathbb{K}\) is a field, \(x\) has an additive inverse \(-x_{\mathbb{K}}\). Note that \(-x_{\mathbb{K}} \in \mathbb{F}\) as well, so \(-x_{\mathbb{K}}\) is an inverse for \(x\) in \(\mathbb{F}\). By the uniqueness of additive inverses in \(\mathbb{F}\), we have that \(-x_{\mathbb{K}} = -x\).

        Similarly, \(x\) has a multiplicative inverse \(x^{-1}_{\mathbb{K}}\) in \(\mathbb{K}\), which is also an inverse of \(x\) with respect to \(\mathbb{F}\). It follows by uniqueness of inverses that \(x ^{-1}_{\mathbb{K}} = x^{-1}\).

        \medskip

        (c):

        Suppose that \(\mathbb{K} \subseteq \mathbb{F}\) is a subfield. We prove each point in order:
        \begin{enumerate}[label=(\roman*)]
            \item By part (a), \(0,1 \in \mathbb{K}\).
            \item This is simply the axiom of closure, which is immediate by assumption.
            \item This is true from part (b).
            \item This is true from part (b).
        \end{enumerate}
        Conversely, suppose that the 4 conditions hold.

        Since \(\mathbb{K}\) has property (ii), it satisfies the axiom of closure.

        To argue commutativity and associativity of elements in \(\mathbb{K}\), notice that every element of \(\mathbb{K}\) is also an element of \(\mathbb{F}\), so they follow the axioms of commutativity, associativity, and distributivity of the field \(\mathbb{F}\).

        Existence of inverses comes directly from (iii) and (iv), and existence of identity element is exactly (i).

        Since \(\mathbb{K}\) satisfies all the field axioms, \(\mathbb{K}\) is indeed a subfield of \(\mathbb{F}\).
    \end{question}
    \newpage
    \begin{question}{5}
        Let \(\mathbb{Q}[\sqrt{-2}] = \{a + b\sqrt{-2} | a,b \in \mathbb{Q}\}\). Prove that if \(\mathbb{K}\) is a subfield of \(\mathbb{C}\) and \(\sqrt{-2} \in \mathbb{K}\), then \(\mathbb{Q}[\sqrt{-2}] \subseteq \mathbb{K}\).
    \end{question}
    \newpage
    \begin{question}{6}
        In this exercise we introduce a new definition:

        **Definition:** Let \(\mathbb{F}\) be a field. The smallest non-negative integer \(n\) so that 
        \(\underbrace{1 + 1 + \cdots + 1}_{n \text{ times}} = 0\)
        is called the characteristic of \(\mathbb{F}\). If no such \(n\) exists, then we say \(\mathbb{F}\) has characteristic 0.

        We denote this non-negative integer by \(\text{char}(\mathbb{F})\).

        For example: \(\mathbb{Z}_3\) has characteristic 3 because \(1 + 1 + 1 = 0\) in \(\mathbb{Z}_3\), but \(1 + 1 \neq 0\) in \(\mathbb{Z}_3\).
        So \(n = 3\) is the smallest integer so that 
        \(\underbrace{1 + 1 + \cdots + 1}_{n \text{ times}} = 0\)
        in \(\mathbb{Z}_3\).

        However, \(\mathbb{Q}\) has characteristic 0, because for any \(n\) we have 
        \(\underbrace{1 + 1 + \cdots + 1}_{n \text{ times}} = n \neq 0\)
        in \(\mathbb{Q}\).

        (a) Prove that \(\text{char}(\mathbb{Z}_p) = p\).

        (b) Prove that \(\text{char}(\mathbb{F})\) must either be prime or 0. (Hint: For the case that \(\text{char}(\mathbb{F})\) is non-zero, use contradiction.)
    \end{question}
    \newpage
    \begin{question}{7}
        In this question we introduce a new definition:

        **Definition:** Let \(f, g \in \mathbb{P}(\mathbb{F})\). We say that a polynomial \(d \in \mathbb{P}(\mathbb{F})\) is a **greatest common divisor** of \(f\) and \(g\) if:

        \begin{itemize}
            \item \(d\) is a divisor of both \(f\) and \(g\), and;
            \item for any other divisor \(d'\) of \(f\) and \(g\), we have \(\deg d \geq \deg d'\).
        \end{itemize}

        (a) Prove that if \(d\) is a common divisor of \(f\) and \(g\), then for all \(a \in \mathbb{F}\), the polynomial \(ad\) is also a common divisor for \(f\) and \(g\). Explain why this shows that there is no "unique" greatest common divisor for \(f\) and \(g\) like there is for integers.

        (b) Prove that if \(d_1, d_2\) are both greatest common divisors for \(f\) and \(g\), then \(d_1 = ad_2\) for some non-zero field element \(a\).

        (c) Prove that we can compute a greatest common divisor for \(f\) and \(g\) like we do for integers: repeatedly apply long division until the remainder is 0, then the last non-zero remainder is a greatest common divisor for \(f\) and \(g\).

        (d) Deduce from (c) that if \(d\) is a greatest common division for \(f\) and \(g\), then we can write \(d = pf + qg\) for some polynomials \(p, q\).

    \end{question}
    \newpage
    \begin{question}{8}
        Apply the procedures in Question 7 to compute a greatest common divisor for the polynomials
        \(f(x) = x^4 + x^2 + 1\), \(g(x) = x^4 + 2x^3 + x^2 + 1 \in \mathbb{P}(\mathbb{Q})\), and express this divisor as a combination
        of \(f\) and \(g\).

        (In particular, you should not try to factor \(f\), \(g\) to find the greatest common divisor, and doing
        so will not receive any credit.)
    \end{question}
    \newpage
    \begin{question}{9}
        Let $p \in \mathbb{P}(\mathbb{C})$ be a polynomial with real coefficients. Prove that if $a$ is a root of $p$, then $\bar{a}$ is a root of $p$. (Hint: Write down an equation that means "$a$ is a root of $p$". Conjugate this equation.)
    \end{question}
    \newpage
    \begin{question}{10}
        Using Question 9 and the Fundamental Theorem of Algebra, prove that the only irreducible 
        polynomials over $\mathbb{R}$ are linear and quadratics with no real roots. Use this to deduce our Theorem from class (Week 2) about the factorization of real polynomials.
    \end{question}
\end{document}